Hashmap/DHashMap/Lemmas.lean
@@ -60,18 +60,34 @@ theorem List.get_congr {l₁ l₂ : List α} {n : Fin l₁.length} (h : l₁ = l
 theorem Nat.lt_of_eq_of_lt {n m k : Nat} : n = m → m < k → n < k :=
   fun h₁ h₂ => h₁ ▸ h₂
 
+/-! # Setting up the infrastructure -/
+
+def bucket [Hashable α] (self : Array (AssocList α β)) (h : 0 < self.size) (k : α) : AssocList α β :=
+  let ⟨i, h⟩ := mkIdx (hash k) h
+  self[i]
+
+def updateBucket [Hashable α] (self : Array (AssocList α β)) (h : 0 < self.size) (k : α)
+    (f : AssocList α β → AssocList α β) : Array (AssocList α β) :=
+  let ⟨i, h⟩ := mkIdx (hash k) h
+  self.uset i (f self[i]) h
+
+@[simp]
+theorem size_updateBucket [Hashable α] {self : Array (AssocList α β)} {h : 0 < self.size} {k : α}
+    {f : AssocList α β → AssocList α β} : (updateBucket self h k f).size = self.size := by
+  simp [updateBucket]
+
 theorem exists_bucket_of_uset [BEq α] [Hashable α]
   (self : Array (AssocList α β)) (i : USize) (hi : i.toNat < self.size) (d : AssocList α β) :
-    ∃ l, self.data.bind AssocList.toList ~ self[i.toNat].toList ++ l ∧
-      (self.uset i d hi).data.bind AssocList.toList ~ d.toList ++ l ∧
+    ∃ l, Raw.toListModel self ~ self[i.toNat].toList ++ l ∧
+      Raw.toListModel (self.uset i d hi) ~ d.toList ++ l ∧
       (∀ [EquivBEq α] [LawfulHashable α],
         IsHashSelf self → ∀ k : α, (mkIdx (hash k) (show 0 < self.size by omega)).1.toNat = i.toNat → l.containsKey k = false) := by
   have h₀ : 0 < self.size := by omega
   obtain ⟨l₁, l₂, h₁, h₂, h₃⟩ := Array.exists_of_update self i d hi
   refine ⟨l₁.bind AssocList.toList ++ l₂.bind AssocList.toList, ?_, ?_, ?_⟩
-  · rw [h₁]
+  · rw [Raw.toListModel, h₁]
     simpa using List.perm_append_comm_assoc _ _ _
-  · rw [h₃]
+  · rw [Raw.toListModel, h₃]
     simpa using List.perm_append_comm_assoc _ _ _
   · intro _ _ h k
     rw [← Decidable.not_imp_not]
@@ -94,13 +110,32 @@ theorem exists_bucket_of_uset [BEq α] [Hashable α]
       rw [Array.size_eq_length_data, h₁, length_append, length_cons]
       omega
 
-theorem exists_bucket [BEq α] [Hashable α]
+theorem exists_bucket_of_update [BEq α] [Hashable α] (m : Array (AssocList α β)) (h : 0 < m.size) (k : α)
+    (f : AssocList α β → AssocList α β) :
+    ∃ l : List (Σ a, β a),
+      Raw.toListModel m ~ (bucket m h k).toList ++ l ∧
+      Raw.toListModel (updateBucket m h k f) ~ (f (bucket m h k)).toList ++ l ∧
+      (∀ [EquivBEq α] [LawfulHashable α], IsHashSelf m → ∀ k', hash k = hash k' → l.containsKey k' = false) := by
+  let idx := mkIdx (hash k) h
+  obtain ⟨l, h₁, h₂, h₃⟩ := exists_bucket_of_uset m idx.1 idx.2 (f m[idx.1])
+  exact ⟨l, h₁, h₂, fun h k' hk' => h₃ h _ (hk' ▸ rfl)⟩
+
+theorem exists_bucket' [BEq α] [Hashable α]
     (self : Array (AssocList α β)) (i : USize) (hi : i.toNat < self.size) :
       ∃ l, self.data.bind AssocList.toList ~ self[i.toNat].toList ++ l ∧
         (∀ [EquivBEq α] [LawfulHashable α], IsHashSelf self → ∀ k,
           (mkIdx (hash k) (show 0 < self.size by omega)).1.toNat = i.toNat → l.containsKey k = false) := by
   obtain ⟨l, h₁, -, h₂⟩ := exists_bucket_of_uset self i hi .nil
   exact ⟨l, h₁, h₂⟩
+
+theorem exists_bucket [BEq α] [Hashable α]
+    (m : Array (AssocList α β)) (h : 0 < m.size) (k : α) :
+    ∃ l : List (Σ a, β a), Raw.toListModel m ~ (bucket m h k).toList ++ l ∧
+      (∀ [EquivBEq α] [LawfulHashable α], IsHashSelf m → ∀ k', hash k = hash k' → l.containsKey k' = false) := by
+  obtain ⟨l, h₁, -, h₂⟩ := exists_bucket_of_update m h k (fun _ => .nil)
+  exact ⟨l, h₁, h₂⟩
+
+/-! # IsHashSelf -/
 
 namespace IsHashSelf
 
@@ -109,25 +144,44 @@ theorem mkArray [BEq α] [Hashable α] {c : Nat} : IsHashSelf (mkArray c (AssocL
   ⟨by simp⟩
 
 theorem uset [BEq α] [Hashable α] {m : Array (AssocList α β)} {i : USize} {h : i.toNat < m.size} {d : AssocList α β}
-    (hd : d.toList.HashesTo i.toNat m.size) (hm : IsHashSelf m) : IsHashSelf (m.uset i d h) := by
+    (hd : m[i].toList.HashesTo i.toNat m.size → d.toList.HashesTo i.toNat m.size) (hm : IsHashSelf m) : IsHashSelf (m.uset i d h) := by
   refine ⟨fun j hj => ?_⟩
   simp only [Array.uset, Array.getElem_set, Array.size_set]
   split
-  · next hij => exact hij ▸ hd
+  · next hij => exact hij ▸ (hd (hm.hashes_to _ _))
   · exact hm.hashes_to j (by simpa using hj)
+
+theorem updateBucket [BEq α] [Hashable α] [EquivBEq α] [LawfulHashable α] {m : Array (AssocList α β)} {h : 0 < m.size} {a : α} {f : AssocList α β → AssocList α β}
+    (hf : ∀ l p, p ∈ (f l).toList → l.toList.containsKey p.1 ∨ hash p.1 = hash a) (hm : IsHashSelf m) : IsHashSelf (updateBucket m h a f) := by
+  rw [DHashMap.updateBucket]
+  refine IsHashSelf.uset (fun h' => ⟨fun _ p hp => ?_⟩) hm
+  rcases hf _ _ hp with (hf|hf)
+  · rw [containsKey_eq_true_iff_exists_mem] at hf
+    rcases hf with ⟨q, hq₁, hq₂⟩
+    rw [← h'.hash_self h _ hq₁, hash_eq hq₂]
+  · rw [hf]
 
 end IsHashSelf
 
 namespace Raw
 
+/-! # size -/
+section size
+
+end size
+
 @[simp]
 theorem size_empty {c} : (empty c : Raw α β).size = 0 := rfl
 
 @[simp]
-theorem toList_empty {c} : (empty c : Raw α β).toList = [] := by
+theorem toListModel_mkArray_nil {c} : toListModel (mkArray c (AssocList.nil : AssocList α β)) = [] := by
   suffices ∀ d, (List.replicate d AssocList.nil).bind AssocList.toList = [] from this _
   intro d
   induction d <;> simp_all
+
+@[simp]
+theorem toListModel_buckets_empty {c} : Raw.toListModel (empty c : Raw α β).buckets = [] :=
+  toListModel_mkArray_nil
 
 theorem ActuallyWF.empty [BEq α] [Hashable α] {c} : (empty c : Raw α β).ActuallyWF where
   buckets_hash_self := by simp [Raw.empty]
@@ -135,20 +189,170 @@ theorem ActuallyWF.empty [BEq α] [Hashable α] {c} : (empty c : Raw α β).Actu
   size_eq := by simp
   distinct := by simp
 
+theorem reinsertAux_eq [Hashable α] (data : { d : Array (AssocList α β) // 0 < d.size }) (a : α) (b : β a) :
+    (Raw.reinsertAux data a b).1 = updateBucket data.1 data.2 a (fun l => l.cons a b) := rfl
+
+theorem reinsertAux_hashSelf [BEq α] [Hashable α] [EquivBEq α] [LawfulHashable α]
+    (data : {d : Array (AssocList α β) // 0 < d.size}) (a : α) (b : β a) (h : IsHashSelf data.1) :
+    IsHashSelf (reinsertAux data a b).1 := by
+  rw [reinsertAux_eq]
+  refine h.updateBucket (fun l p hp => ?_)
+  simp only [AssocList.toList_cons, mem_cons] at hp
+  rcases hp with (rfl|hp)
+  · exact Or.inr rfl
+  · exact Or.inl (containsKey_of_mem hp)
+
+theorem reinsertAux_toListModel [BEq α] [Hashable α] [EquivBEq α] [LawfulHashable α]
+    (data : {d : Array (AssocList α β) // 0 < d.size}) (a : α) (b : β a) :
+    toListModel (reinsertAux data a b).1 ~ ⟨a, b⟩ :: toListModel data.1 := by
+  rw [reinsertAux_eq]
+  obtain ⟨l, h₁, h₂, -⟩ := exists_bucket_of_update data.1 data.2 a (fun l => l.cons a b)
+  exact h₂.trans (by simpa using h₁.symm)
+
+theorem expand.foldl_hashSelf [BEq α] [Hashable α] [EquivBEq α] [LawfulHashable α] (l : AssocList α β) (target : { d : Array (AssocList α β) // 0 < d.size }) :
+    IsHashSelf target.1 → IsHashSelf (l.foldl reinsertAux target).1 := by
+  induction l generalizing target
+  · simp [AssocList.foldl, AssocList.foldlM, Id.run]
+  · next k v _ ih => exact fun h => ih _ (reinsertAux_hashSelf _ _ _ h)
+
+theorem expand.foldl_toListModel [BEq α] [Hashable α] [EquivBEq α] [LawfulHashable α] (l : AssocList α β)
+    (target : { d : Array (AssocList α β) // 0 < d.size }) :
+    toListModel (l.foldl reinsertAux target).1 ~ l.toList ++ toListModel target.1 := by
+  induction l generalizing target
+  · simp
+  · next k v t ih =>
+    skip
+    simp at ih
+    simp
+    refine (ih _).trans ?_
+    refine ((reinsertAux_toListModel _ _ _).append_left _).trans perm_middle
+
+theorem expand.go_pos [Hashable α] {i : Nat} {source : Array (AssocList α β)} {target : { d : Array (AssocList α β) // 0 < d.size }}
+    (h : i < source.size) : expand.go i source target =
+      go (i + 1) (source.set ⟨i, h⟩ .nil) ((source.get ⟨i, h⟩).foldl reinsertAux target) := by
+  rw [expand.go]
+  simp only [h, dite_true]
+
+theorem expand.go_neg [Hashable α] {i : Nat} {source : Array (AssocList α β)} {target : { d : Array (AssocList α β) // 0 < d.size}}
+    (h : ¬i < source.size) : expand.go i source target = target := by
+  rw [expand.go]
+  simp only [h, dite_false]
+
+theorem expand.hashSelf [BEq α] [Hashable α] [LawfulHashable α] [EquivBEq α] {buckets : {d : Array (AssocList α β) // 0 < d.size}} :
+    IsHashSelf (expand buckets).1 := by
+  rw [expand]
+  apply go
+  simp only [IsHashSelf.mkArray]
+  where
+    go (i) (source : Array (AssocList α β)) (target : {d : Array (AssocList α β) // 0 < d.size}) :
+        IsHashSelf target.1 → IsHashSelf (expand.go i source target).1 := by
+      induction i, source, target using expand.go.induct
+      · next i source target hi _ es newSource newTarget ih =>
+        simp only [newSource, newTarget, es] at *
+        rw [expand.go_pos hi]
+        refine ih ∘ ?_
+        exact expand.foldl_hashSelf _ _
+      · next i source target hi =>
+        rw [expand.go_neg hi]
+        exact id
+
+theorem expand.toListModel [BEq α] [Hashable α] [LawfulHashable α] [EquivBEq α] {buckets : {d : Array (AssocList α β) // 0 < d.size}} :
+    toListModel (expand buckets).1 ~ toListModel buckets.1 := by
+  rw [expand]
+  refine (go _ _ _).trans ?_
+  rw [drop_zero, toListModel_mkArray_nil, append_nil, Raw.toListModel]
+  where
+    go (i) (source : Array (AssocList α β)) (target : {d : Array (AssocList α β) // 0 < d.size}) :
+        Raw.toListModel (expand.go i source target).1 ~ (source.data.drop i).bind AssocList.toList ++ Raw.toListModel target.1 := by
+      induction i, source, target using expand.go.induct
+      · next i source target hi _ es newSource newTarget ih =>
+        simp only [newSource, newTarget, es] at *
+        rw [expand.go_pos hi]
+        refine ih.trans ?_
+        rw [Array.size_eq_length_data] at hi
+        rw [List.drop_eq_get_cons hi, List.cons_bind, Array.data_set, List.drop_set_of_lt _ _ (Nat.lt_succ_self i),
+          Array.get_eq_getElem, Array.getElem_eq_data_get]
+        refine ((expand.foldl_toListModel _ _).append_left _).trans ?_
+        simp only [Nat.succ_eq_add_one, Array.data_length, append_assoc]
+        exact List.perm_append_comm_assoc _ _ _
+      · next i source target hi =>
+        rw [expand.go_neg hi]
+        rw [Array.size_eq_length_data, Nat.not_lt, ← List.drop_eq_nil_iff_le] at hi
+        simp [hi]
+
+theorem toListModel_expandIfNecessary [BEq α] [Hashable α] [EquivBEq α] [LawfulHashable α] (m : {m : Raw α β // 0 < m.buckets.size}) :
+    toListModel (expandIfNecessary m).1.2 ~ toListModel m.1.2 := by
+  rw [Raw.expandIfNecessary]
+  dsimp
+  split
+  · exact Perm.refl _
+  · dsimp
+    exact expand.toListModel
+
+theorem ActuallyWF.expandIfNecessary [BEq α] [Hashable α] [EquivBEq α] [LawfulHashable α] (m : { m : Raw α β // 0 < m.buckets.size })
+    (h : m.1.ActuallyWF) : (expandIfNecessary m).1.ActuallyWF := by
+  rw [Raw.expandIfNecessary]
+  dsimp
+  split
+  · exact h
+  · let ⟨⟨size, buckets⟩, hm⟩ := m
+    have := expand.toListModel (buckets := ⟨buckets, hm⟩)
+    dsimp at this
+    refine ⟨?_, ?_, ?_, ?_⟩
+    · simpa using expand.hashSelf
+    · simpa using (expand _).2
+    · refine h.size_eq.trans ?_
+      simpa using this.symm.length_eq
+    · simpa using WF_of_perm this h.distinct
+
+def replace [BEq α] [Hashable α] (m : { m : Raw α β // 0 < m.buckets.size }) (a : α) (b : β a) : Raw α β :=
+  ⟨m.1.size, updateBucket m.1.buckets m.2 a (fun l => l.replace a b)⟩
+
+theorem toListModel_replace [BEq α] [Hashable α] [EquivBEq α] [LawfulHashable α] (m : { m : Raw α β // 0 < m.buckets.size })
+    (h : m.1.ActuallyWF) (a : α) (b : β a) : toListModel (replace m a b).buckets ~ (toListModel m.1.2).replaceEntry a b := by
+  rw [replace]
+  dsimp only
+  obtain ⟨l, h₁, h₂, h₃⟩ := exists_bucket_of_update m.1.buckets m.2 a (fun l => l.replace a b)
+  refine h₂.trans (Perm.trans ?_ (replaceEntry_of_perm _ _ h.distinct h₁).symm)
+  rw [AssocList.toList_replace, replaceEntry_append_of_containsKey_right_eq_false]
+  apply h₃ h.buckets_hash_self _ rfl
+
+theorem isHashSelf_replace [BEq α] [Hashable α] [EquivBEq α] [LawfulHashable α] (m : { m : Raw α β // 0 < m.buckets.size })
+    (h : m.1.ActuallyWF) (a : α) (b : β a) : IsHashSelf (replace m a b).buckets := by
+  rw [replace]
+  dsimp only
+  apply h.buckets_hash_self.updateBucket (fun l p hp => ?_)
+  exact Or.inl (by simpa using containsKey_of_mem hp)
+
+theorem ActuallyWF.replace [BEq α] [Hashable α] [EquivBEq α] [LawfulHashable α] (m : { m : Raw α β // 0 < m.buckets.size })
+    (h : m.1.ActuallyWF) (a : α) (b : β a) : (replace m a b).ActuallyWF where
+  buckets_hash_self := isHashSelf_replace m h a b
+  buckets_size := by simpa [Raw.replace] using h.buckets_size
+  size_eq := h.size_eq.trans (Eq.trans length_replaceEntry.symm (toListModel_replace _ h _ _).length_eq.symm)
+  distinct := WF_of_perm (toListModel_replace _ h _ _) (WF_replaceEntry h.distinct)
+
+-- def insertNoResize [Hashable α] [BEq α] (data : {m : Raw α β // 0 < m.buckets.size})
+
+-- theorem insertWellFormed_eq [Hashable α] [BEq α] {data : { m : Raw α β // 0 < m.buckets.size }} {a : α} {b : β a}
+
+theorem findEntry?wellFormed_eq [Hashable α] [BEq α] (data : { m : Raw α β // 0 < m.buckets.size }) (a : α) :
+    Raw.findEntry?WellFormed data a = (bucket data.1.buckets data.2 a).findEntry? a := rfl
+
 theorem bucket_contains_eq_containsKey [BEq α] [Hashable α] [EquivBEq α] [LawfulHashable α] {m : Raw α β} (hm : m.ActuallyWF) {a : α} :
-    haveI h : (mkIdx (hash a) hm.buckets_size).1.toNat < m.buckets.size := (mkIdx (hash a) hm.buckets_size).2
-    (m.buckets[(mkIdx (hash a) hm.buckets_size).1.toNat]'h).contains a = m.toList.containsKey a := by
-  obtain ⟨l, hl, hlk⟩ := exists_bucket m.buckets (mkIdx (hash a) hm.buckets_size).1 (mkIdx (hash a) hm.buckets_size).2
+    (bucket m.buckets hm.buckets_size a).contains a = (Raw.toListModel m.buckets).containsKey a := by
+  obtain ⟨l, hl, hlk⟩ := exists_bucket m.buckets hm.buckets_size a
   refine Eq.trans ?_ (List.containsKey_of_perm (WF_of_perm hl.symm hm.distinct) hl.symm)
   rw [AssocList.contains_eq, List.containsKey_append_of_not_contains_right]
   exact hlk hm.buckets_hash_self _ rfl
 
-theorem size_insertWellFormed [BEq α] [Hashable α] [EquivBEq α] [LawfulHashable α] {m : { m : Raw α β // 0 < m.buckets.size }} {a : α} {b : β a} :
+theorem size_insertWellFormed [BEq α] [Hashable α] [EquivBEq α] [LawfulHashable α] {m : { m : Raw α β // 0 < m.buckets.size }}
+    (hm : m.1.ActuallyWF) {a : α} {b : β a} :
     (insertWellFormed m a b).1.1.size = if m.1.toList.containsKey a then m.1.size else m.1.size + 1 := by
   rw [insertWellFormed]
-  dsimp
-  rw [bucket_contains_eq_containsKey]
-  sorry
+  dsimp only [Array.ugetElem_eq_getElem, Array.uset]
+  rw [bucket_contains_eq_containsKey hm]
+  split <;> try rfl
+  split <;> rfl
 
 theorem findEntry?WellFormed_eq_findEntry_toList [BEq α] [EquivBEq α] [Hashable α] [LawfulHashable α]
     (m : { m : Raw α β // 0 < m.buckets.size }) (h : m.1.ActuallyWF) (a : α) :
